wip

crypto/bignum/x25519/Hacl.Bignum.Fsquare.fst
@@ -13,7 +13,25 @@ open Hacl.Bignum.Fproduct
 open Hacl.Spec.Bignum.Fsquare
 
 
-#set-options "--z3rlimit 500 --initial_fuel 0 --max_fuel 0"
+#set-options "--z3rlimit 50 --initial_fuel 0 --max_fuel 0"
+
+private inline_for_extraction val upd_5:
+  tmp:felem_wide -> s0:wide -> s1:wide -> s2:wide -> s3:wide -> s4:wide ->
+  Stack unit
+    (requires (fun h -> live h tmp))
+    (ensures (fun h0 _ h1 -> live h1 tmp /\ as_seq h1 tmp == seq_upd_5 s0 s1 s2 s3 s4
+      /\ modifies_1 tmp h0 h1))
+private inline_for_extraction let upd_5 tmp s0 s1 s2 s3 s4 =
+  tmp.(0ul) <- s0;
+  tmp.(1ul) <- s1;
+  tmp.(2ul) <- s2;
+  tmp.(3ul) <- s3;
+  tmp.(4ul) <- s4;
+  let h1 = ST.get() in
+  Seq.lemma_eq_intro (as_seq h1 tmp) (seq_upd_5 s0 s1 s2 s3 s4)
+
+
+#set-options "--z3rlimit 50 --initial_fuel 0 --max_fuel 0"
 
 private val fsquare__:
   tmp:felem_wide ->
@@ -24,6 +42,7 @@ private val fsquare__:
       /\ fsquare_pre_ (as_seq h0 output)
       /\ as_seq h1 tmp == fsquare_spec_ (as_seq h0 output)))
 private let fsquare__ tmp output =
+  let h0 = ST.get() in
   let r0 = output.(0ul) in
   let r1 = output.(1ul) in
   let r2 = output.(2ul) in
@@ -40,11 +59,15 @@ private let fsquare__ tmp output =
   let s2 =  computation_3 r0 r1 r2 r3 r4 d4 d0 in
   let s3 = computation_4 r0 r1 r2 r3 r4 d419 d0 d1 in
   let s4 = computation_5 r0 r1 r2 r3 r4 d0 d1 in
-  tmp.(0ul) <- s0;
-  tmp.(1ul) <- s1;
-  tmp.(2ul) <- s2;
-  tmp.(3ul) <- s3;
-  tmp.(4ul) <- s4
+  upd_5 tmp s0 s1 s2 s3 s4;
+  let h1 = ST.get() in
+  Seq.lemma_eq_intro (as_seq h1 tmp) (fsquare_spec_ (as_seq h0 output))
+
+  (* tmp.(0ul) <- s0; *)
+  (* tmp.(1ul) <- s1; *)
+  (* tmp.(2ul) <- s2; *)
+  (* tmp.(3ul) <- s3; *)
+  (* tmp.(4ul) <- s4 *)
   (* tmp.(0ul) <- ( r0) *^ r0 +^ ( d4) *^ r1 +^ (( d2) *^ (r3     )); *)
   (* tmp.(1ul) <- ( d0) *^ r1 +^ ( d4) *^ r2 +^ (( r3) *^ (Hacl.Bignum.Limb.(r3 *^ (uint64_to_limb 19uL)))); *)
   (* tmp.(2ul) <- ( d0) *^ r2 +^ ( r1) *^ r1 +^ (( d4) *^ (r3     )); *)
@@ -73,43 +96,48 @@ private let fsquare_ tmp output =
   carry_0_to_1 output
 
 
-#set-options "--z3rlimit 5 --initial_fuel 1 --max_fuel 1"
+#set-options "--z3rlimit 100 --initial_fuel 1 --max_fuel 1"
 
 private val fsquare_times_:
   input:felem ->
   tmp:felem_wide{disjoint input tmp} ->
-  count:FStar.UInt32.t ->
+  count:FStar.UInt32.t{FStar.UInt32.v count > 0} ->
   Stack unit
-    (requires (fun h -> live h input /\ live h tmp /\ Hacl.Spec.EC.AddAndDouble.red_52 (as_seq h input)))
+    (requires (fun h -> live h input /\ live h tmp /\ Hacl.Spec.EC.AddAndDouble.red_5413 (as_seq h input)))
     (ensures (fun h0 _ h1 -> live h0 input /\ live h1 input /\ live h1 tmp /\ modifies_2 input tmp h0 h1
       /\ Hacl.Spec.EC.AddAndDouble.red_5413 (as_seq h0 input)
       /\ Hacl.Spec.EC.AddAndDouble.red_513 (as_seq h1 input)
       /\ as_seq h1 input == fsquare_times_tot (as_seq h0 input) (FStar.UInt32.v count)))
 private let rec fsquare_times_ output tmp count =
-  if FStar.UInt32.(count =^ 0ul) then ()
+  if FStar.UInt32.(count =^ 1ul) then (
+    let h0 = ST.get() in
+    fsquare_5413_is_fine (as_seq h0 output);
+    fsquare_  tmp output
+  )
   else (
     let i = FStar.UInt32.(count -^ 1ul) in
+    cut (FStar.UInt32.v i > 0);
     let h0 = ST.get() in
-    fsquare_53_is_fine (as_seq h0 output);
+    fsquare_5413_is_fine (as_seq h0 output);
     fsquare_  tmp output;
     let h1 = ST.get() in
-    cut (Hacl.Spec.EC.AddAndDouble.red_52 (as_seq h1 output));
+    cut (Hacl.Spec.EC.AddAndDouble.red_5413 (as_seq h1 output));
     cut (modifies_2 tmp output h0 h1);
-    fsquare_times_ output tmp (FStar.UInt32.(count -^ 1ul))
+    fsquare_times_ output tmp i
   )
 
 
-#set-options "--z3rlimit 5 --initial_fuel 0 --max_fuel 0"
+#set-options "--z3rlimit 10 --initial_fuel 0 --max_fuel 0"
 
 val fsquare_times:
   output:felem ->
   input:felem{disjoint output input} ->
-  count:FStar.UInt32.t ->
+  count:FStar.UInt32.t{FStar.UInt32.v count > 0} ->
   Stack unit
-    (requires (fun h -> live h output /\ live h input /\ Hacl.Spec.EC.AddAndDouble.red_52 (as_seq h input)))
+    (requires (fun h -> live h output /\ live h input /\ Hacl.Spec.EC.AddAndDouble.red_5413 (as_seq h input)))
     (ensures (fun h0 _ h1 -> live h0 output /\ live h1 output /\ live h0 input /\ modifies_1 output h0 h1
-      /\ Hacl.Spec.EC.AddAndDouble.red_52 (as_seq h0 input)
-      /\ Hacl.Spec.EC.AddAndDouble.red_52 (as_seq h1 output)
+      /\ Hacl.Spec.EC.AddAndDouble.red_5413 (as_seq h0 input)
+      /\ Hacl.Spec.EC.AddAndDouble.red_513 (as_seq h1 output)
       /\ (as_seq h1 output) == fsquare_times_tot (as_seq h0 input) (FStar.UInt32.v count)))
 let fsquare_times output input count =
   push_frame();
