crypto/bignum/x25519/Hacl.EC.AddAndDouble.fst
@@ -27,8 +27,16 @@ let all_disjoint (ppx:felem) (ppz:felem) (ppqx:felem) (ppqz:felem)
   /\ disjoint pqx pqz /\ disjoint pqx qx
   /\ disjoint pqz qx
 
+let same_frame (ppx:felem) (ppz:felem) (ppqx:felem) (ppqz:felem)
+               (px:felem) (pz:felem) (pqx:felem) (pqz:felem) : GTot Type0 =
+  frameOf ppx = frameOf ppz /\ frameOf ppx = frameOf ppqx /\ frameOf ppx = frameOf ppqz
+  /\ frameOf ppx = frameOf px /\ frameOf ppx = frameOf pz /\ frameOf ppx = frameOf pqx
+  /\ frameOf pqx = frameOf pqz
+
 
 inline_for_extraction let red_513 s = Hacl.Spec.EC.AddAndDouble.red_513 s
+inline_for_extraction let red_53 s = Hacl.Spec.EC.AddAndDouble.red_53 s
+inline_for_extraction let red_5413 s = Hacl.Spec.EC.AddAndDouble.red_5413 s
 
 
 (* val fmonty_1: *)
@@ -154,7 +162,392 @@ inline_for_extraction let red_513 s = Hacl.Spec.EC.AddAndDouble.red_513 s
 (* ********************************************************************************* *)
 (* ********************************************************************************* *)
 
+#set-options "--initial_fuel 0 --max_fuel 0 --z3rlimit 10"
+
+
+val fmonty__1:
+  tmp:buffer limb{length tmp = 40} ->
+  ppx:felem -> ppz:felem -> ppqx:felem -> ppqz:felem ->
+  px:felem -> pz:felem -> pqx:felem -> pqz:felem ->
+  qx:felem -> Stack unit
+    (requires (fun h ->
+      live h ppx /\ live h ppz /\ live h ppqx /\ live h ppqz
+      /\ live h px /\ live h pz /\ live h pqx /\ live h pqz
+      /\ live h qx /\ live h tmp
+      /\ red_513 (as_seq h px) /\ red_513 (as_seq h pz) /\ red_513 (as_seq h pqx) /\ red_513 (as_seq h pqz)
+      /\ red_513 (as_seq h qx)
+      /\ all_disjoint ppx ppz ppqx ppqz px pz pqx pqz qx
+      /\ same_frame ppx ppz ppqx ppqz px pz pqx pqz
+      /\ frameOf ppx <> frameOf tmp /\ frameOf ppx <> frameOf qx /\ frameOf qx <> frameOf tmp))
+    (ensures (fun h0 _ h1 ->
+      live h0 ppx /\ live h0 ppz /\ live h0 ppqx /\ live h0 ppqz
+      /\ live h0 px /\ live h0 pz /\ live h0 pqx /\ live h0 pqz
+      /\ live h0 qx /\ live h0 tmp
+      /\ live h1 ppx /\ live h1 ppz /\ live h1 ppqx /\ live h1 ppqz
+      /\ live h1 px /\ live h1 pz /\ live h1 pqx /\ live h1 pqz
+      /\ live h1 tmp /\ live h1 qx
+      /\ red_513 (as_seq h0 px) /\ red_513 (as_seq h0 pz) /\ red_513 (as_seq h0 pqx) /\ red_513 (as_seq h0 pqz)
+      /\ red_513 (as_seq h0 qx)
+      /\ all_disjoint ppx ppz ppqx ppqz px pz pqx pqz qx
+      /\ red_53 (as_seq h1 px) /\ red_5413 (as_seq h1 pz)
+      /\ red_513 (as_seq h1 (Buffer.sub tmp 25ul 5ul))
+      /\ red_513 (as_seq h1 (Buffer.sub tmp 30ul 5ul))
+      /\ (as_seq h1 px, as_seq h1 pz, as_seq h1 (Buffer.sub tmp 25ul 5ul), as_seq h1 (Buffer.sub tmp 30ul 5ul)) == fmonty_tot_1 (as_seq h0 px) (as_seq h0 pz) (as_seq h0 pqx) (as_seq h0 pqz) (as_seq h0 qx)
+      /\ as_seq h1 qx == as_seq h0 qx
+    ))
 #set-options "--initial_fuel 0 --max_fuel 0 --z3rlimit 100"
+let fmonty__1 buf x2 z2 x3 z3 x z xprime zprime qx =
+  let origx      = Buffer.sub buf 0ul  5ul in
+  let origxprime = Buffer.sub buf 5ul  5ul in
+  let zzz        = Buffer.sub buf 10ul 5ul in
+  let xx         = Buffer.sub buf 15ul 5ul in
+  let zz         = Buffer.sub buf 20ul 5ul in
+  let xxprime    = Buffer.sub buf 25ul 5ul in
+  let zzprime    = Buffer.sub buf 30ul 5ul in
+  let zzzprime   = Buffer.sub buf 35ul 5ul in
+  let h0 = ST.get() in
+  blit x 0ul origx 0ul 5ul;
+  let h1 = ST.get() in
+  Hacl.Spec.Bignum.Fmul.lemma_whole_slice (as_seq h0 x);
+  Hacl.Spec.Bignum.Fmul.lemma_whole_slice (as_seq h1 origx);
+  Hacl.Spec.EC.AddAndDouble.fsum_513_is_53 (as_seq h1 x) (as_seq h1 z);
+  fsum x z; // x < x + z
+  let h2 = ST.get() in
+  Hacl.Spec.EC.AddAndDouble.lemma_fdifference_unrolled'' (as_seq h2 z) (as_seq h2 origx);
+  Hacl.Spec.EC.AddAndDouble.lemma_fdifference_unrolled''' (as_seq h2 z) (as_seq h2 origx);
+  fdifference z origx; // z <- 8p + x - z
+  let h3 = ST.get() in
+  blit xprime 0ul origxprime 0ul 5ul;
+  let h4 = ST.get() in
+  Hacl.Spec.Bignum.Fmul.lemma_whole_slice (as_seq h3 xprime);
+  Hacl.Spec.Bignum.Fmul.lemma_whole_slice (as_seq h4 origxprime);
+  Hacl.Spec.EC.AddAndDouble.fsum_513_is_53 (as_seq h4 xprime) (as_seq h4 zprime);
+  fsum xprime zprime; // xprime <- xprime + zprime
+  let h5 = ST.get() in
+  Hacl.Spec.EC.AddAndDouble.lemma_fdifference_unrolled'' (as_seq h5 zprime) (as_seq h5 origxprime);
+  fdifference zprime origxprime; // zprime <- 8p + xprime - zprime
+  let h6 = ST.get() in
+  Hacl.Spec.EC.AddAndDouble.fmul_53_55_is_fine (as_seq h6 xprime) (as_seq h6 z);
+  fmul xxprime xprime z; // xxprime <- sum * sub
+  let h7 = ST.get() in
+  Hacl.Spec.EC.AddAndDouble.fmul_53_55_is_fine (as_seq h7 x) (as_seq h7 zprime);
+  fmul zzprime x zprime; // zzprime <- sum * sub
+  ()
+
+
+val fmonty__2:
+  tmp:buffer limb{length tmp = 40} ->
+  ppx:felem -> ppz:felem -> ppqx:felem -> ppqz:felem ->
+  px:felem -> pz:felem -> pqx:felem -> pqz:felem ->
+  qx:felem -> Stack unit
+    (requires (fun h ->
+      live h ppx /\ live h ppz /\ live h ppqx /\ live h ppqz
+      /\ live h px /\ live h pz /\ live h pqx /\ live h pqz
+      /\ live h qx /\ live h tmp
+      /\ red_513 (as_seq h qx)
+      /\ red_53 (as_seq h px) /\ red_5413 (as_seq h pz)
+      /\ red_513 (as_seq h (Buffer.sub tmp 25ul 5ul))
+      /\ red_513 (as_seq h (Buffer.sub tmp 30ul 5ul))
+      /\ all_disjoint ppx ppz ppqx ppqz px pz pqx pqz qx
+      /\ same_frame ppx ppz ppqx ppqz px pz pqx pqz
+      /\ frameOf ppx <> frameOf tmp /\ frameOf ppx <> frameOf qx /\ frameOf qx <> frameOf tmp))
+    (ensures (fun h0 _ h1 ->
+      let xx         = Buffer.sub tmp 15ul 5ul in
+      let zz         = Buffer.sub tmp 20ul 5ul in
+      let xxprime    = Buffer.sub tmp 25ul 5ul in
+      let zzprime    = Buffer.sub tmp 30ul 5ul in
+      live h0 ppx /\ live h0 ppz /\ live h0 ppqx /\ live h0 ppqz
+      /\ live h0 px /\ live h0 pz /\ live h0 pqx /\ live h0 pqz
+      /\ live h0 qx /\ live h0 tmp
+      /\ live h1 ppx /\ live h1 ppz /\ live h1 ppqx /\ live h1 ppqz
+      /\ live h1 px /\ live h1 pz /\ live h1 pqx /\ live h1 pqz
+      /\ live h1 tmp /\ live h1 qx
+      /\ red_513 (as_seq h0 qx)
+      /\ red_53 (as_seq h0 px) /\ red_5413 (as_seq h0 pz)
+      /\ red_513 (as_seq h0 xxprime)
+      /\ red_513 (as_seq h0 zzprime)
+      /\ all_disjoint ppx ppz ppqx ppqz px pz pqx pqz qx
+      /\ red_513 (as_seq h1 xx) /\ red_513 (as_seq h1 zz)
+      /\ red_513 (as_seq h1 ppqx) /\ red_513 (as_seq h1 ppqz)
+      /\ (as_seq h1 ppqx, as_seq h1 ppqz, as_seq h1 xx, as_seq h1 zz) ==
+          fmonty_tot_2 (as_seq h0 px) (as_seq h0 pz) (as_seq h0 qx) (as_seq h0 xxprime)
+                      (as_seq h0 zzprime)
+      /\ as_seq h1 qx == as_seq h0 qx
+    ))
+#set-options "--initial_fuel 0 --max_fuel 0 --z3rlimit 500"
+let fmonty__2 buf x2 z2 x3 z3 x z xprime zprime qx =
+  let origx      = Buffer.sub buf 0ul  5ul in
+  let origxprime = Buffer.sub buf 5ul  5ul in
+  let zzz        = Buffer.sub buf 10ul 5ul in
+  let xx         = Buffer.sub buf 15ul 5ul in
+  let zz         = Buffer.sub buf 20ul 5ul in
+  let xxprime    = Buffer.sub buf 25ul 5ul in
+  let zzprime    = Buffer.sub buf 30ul 5ul in
+  let zzzprime   = Buffer.sub buf 35ul 5ul in
+  let h8 = ST.get() in
+  (* cut (red_513 (as_seq h8 xxprime)); *)
+  (* cut (red_513 (as_seq h8 zzprime)); *)
+  blit xxprime 0ul origxprime 0ul 5ul;
+  let h9 = ST.get() in
+  Hacl.Spec.Bignum.Fmul.lemma_whole_slice (as_seq h8 xxprime);
+  Hacl.Spec.Bignum.Fmul.lemma_whole_slice (as_seq h9 origxprime);
+  no_upd_lemma_1 h8 h9 origxprime zzprime;
+  no_upd_lemma_1 h8 h9 origxprime xxprime;
+  Hacl.Spec.EC.AddAndDouble.fsum_513_is_53 (as_seq h9 xxprime) (as_seq h9 zzprime);
+  fsum xxprime zzprime; // xxprime <- sum xxprime' = xxprime + zzprime
+  let h10 = ST.get() in
+  no_upd_lemma_1 h9 h10 xxprime zzprime;
+  no_upd_lemma_1 h9 h10 xxprime origxprime;
+  Hacl.Spec.EC.AddAndDouble.lemma_fdifference_unrolled''' (as_seq h10 zzprime) (as_seq h10 origxprime);
+  fdifference zzprime origxprime; // zzprime <- sub zzprime' = xxprime - zzprime
+  let h11 = ST.get() in
+  no_upd_lemma_1 h10 h11 zzprime xxprime;
+  lemma_53_is_5413 (as_seq h11 xxprime);
+  Hacl.Spec.Bignum.Fsquare.fsquare_5413_is_fine (as_seq h11 xxprime);
+  fsquare_times x3 xxprime 1ul; // sum sum x3 = xxprime' * xxprime'
+  let h12 = ST.get() in
+  no_upd_lemma_1 h11 h12 x3 zzprime;
+  (* lemma_53_is_5413 (as_seq h12 zzprime); *)
+  Hacl.Spec.Bignum.Fsquare.fsquare_5413_is_fine (as_seq h12 zzprime);
+  fsquare_times zzzprime zzprime 1ul; // sub sub zzzprime = zzprime' * zzprime'
+  let h13 = ST.get() in
+  no_upd_lemma_1 h8 h9 origxprime qx;
+  no_upd_lemma_1 h9 h10 xxprime qx;
+  no_upd_lemma_1 h10 h11 zzprime qx;
+  no_upd_lemma_1 h11 h12 x3 qx;
+  no_upd_lemma_1 h12 h13 zzzprime qx;
+  lemma_513_is_53 (as_seq h13 zzzprime);
+  lemma_513_is_55 (as_seq h13 qx);
+  Hacl.Spec.EC.AddAndDouble.fmul_53_55_is_fine (as_seq h13 zzzprime) (as_seq h13 qx);
+  fmul z3 zzzprime qx; // z3 = zzzprime * qx
+  let h14 = ST.get() in
+  no_upd_lemma_1 h8 h9 origxprime x;
+  no_upd_lemma_1 h9 h10 xxprime x;
+  no_upd_lemma_1 h10 h11 zzprime x;
+  no_upd_lemma_1 h11 h12 x3 x;
+  no_upd_lemma_1 h12 h13 zzzprime x;
+  no_upd_lemma_1 h13 h14 z3 x;
+  lemma_53_is_5413 (as_seq h14 x);
+  Hacl.Spec.Bignum.Fsquare.fsquare_5413_is_fine (as_seq h14 x);
+  fsquare_times xx x 1ul; // sum red xx = x * x
+  let h15 = ST.get() in
+  no_upd_lemma_1 h8 h9 origxprime z;
+  no_upd_lemma_1 h9 h10 xxprime z;
+  no_upd_lemma_1 h10 h11 zzprime z;
+  no_upd_lemma_1 h11 h12 x3 z;
+  no_upd_lemma_1 h12 h13 zzzprime z;
+  no_upd_lemma_1 h13 h14 z3 z;
+  no_upd_lemma_1 h14 h15 xx z;
+  Hacl.Spec.Bignum.Fsquare.fsquare_5413_is_fine (as_seq h15 z);
+  fsquare_times zz z 1ul; // red sub zz = z * z
+  ()
+
+
+#set-options "--initial_fuel 0 --max_fuel 0 --z3rlimit 10"
+
+val fmonty__3:
+  tmp:buffer limb{length tmp = 40} ->
+  ppx:felem -> ppz:felem -> ppqx:felem -> ppqz:felem ->
+  px:felem -> pz:felem -> pqx:felem -> pqz:felem ->
+  qx:felem -> Stack unit
+    (requires (fun h ->
+      let xx         = Buffer.sub tmp 15ul 5ul in
+      let zz         = Buffer.sub tmp 20ul 5ul in
+      live h ppx /\ live h ppz /\ live h ppqx /\ live h ppqz
+      /\ live h px /\ live h pz /\ live h pqx /\ live h pqz
+      /\ live h qx /\ live h tmp
+      /\ red_513 (as_seq h ppqx) /\ red_513 (as_seq h ppqz)
+      /\ red_513 (as_seq h xx) /\ red_513 (as_seq h zz)
+      /\ red_513 (as_seq h qx)
+      /\ all_disjoint ppx ppz ppqx ppqz px pz pqx pqz qx
+      /\ same_frame ppx ppz ppqx ppqz px pz pqx pqz
+      /\ frameOf ppx <> frameOf tmp /\ frameOf ppx <> frameOf qx /\ frameOf qx <> frameOf tmp))
+    (ensures (fun h0 _ h1 ->
+      let xx         = Buffer.sub tmp 15ul 5ul in
+      let zz         = Buffer.sub tmp 20ul 5ul in
+      live h0 ppx /\ live h0 ppz /\ live h0 ppqx /\ live h0 ppqz
+      /\ live h0 px /\ live h0 pz /\ live h0 pqx /\ live h0 pqz
+      /\ live h0 qx /\ live h0 tmp
+      /\ live h1 ppx /\ live h1 ppz /\ live h1 ppqx /\ live h1 ppqz
+      /\ live h1 px /\ live h1 pz /\ live h1 pqx /\ live h1 pqz
+      /\ live h1 tmp /\ live h1 qx
+      /\ red_513 (as_seq h0 ppqx) /\ red_513 (as_seq h0 ppqz)
+      /\ red_513 (as_seq h0 xx) /\ red_513 (as_seq h0 zz)
+      /\ red_513 (as_seq h0 qx)
+      /\ all_disjoint ppx ppz ppqx ppqz px pz pqx pqz qx
+      /\ red_513 (as_seq h1 ppx) /\ red_513 (as_seq h1 ppz)
+      /\ red_513 (as_seq h1 ppqx) /\ red_513 (as_seq h1 ppqz)
+      /\ (as_seq h1 ppx, as_seq h1 ppz, as_seq h1 ppqx, as_seq h1 ppqz) ==
+          fmonty_tot_3 (as_seq h0 ppqx) (as_seq h0 ppqz) (as_seq h0 xx) (as_seq h0 zz)
+      /\ as_seq h1 qx == as_seq h0 qx
+    ))
+
+let lemma_5413_is_55 (s:seqelem{red_5413 s}) : Lemma (Hacl.Spec.EC.AddAndDouble.red_55 s) = ()
+
+#set-options "--initial_fuel 0 --max_fuel 0 --z3rlimit 1000"
+let fmonty__3 buf x2 z2 x3 z3 x z xprime zprime qx =
+  let origx      = Buffer.sub buf 0ul  5ul in
+  let origxprime = Buffer.sub buf 5ul  5ul in
+  let zzz        = Buffer.sub buf 10ul 5ul in
+  let xx         = Buffer.sub buf 15ul 5ul in
+  let zz         = Buffer.sub buf 20ul 5ul in
+  let xxprime    = Buffer.sub buf 25ul 5ul in
+  let zzprime    = Buffer.sub buf 30ul 5ul in
+  let zzzprime   = Buffer.sub buf 35ul 5ul in
+  let h16 = ST.get() in
+  lemma_513_is_53 (as_seq h16 xx);
+  lemma_513_is_55 (as_seq h16 zz);
+  Hacl.Spec.EC.AddAndDouble.fmul_53_55_is_fine (as_seq h16 xx)  (as_seq h16 zz);
+  fmul x2 xx zz; // red red
+  let h17 = ST.get() in
+  no_upd_lemma_1 h16 h17 x2 zz;
+  no_upd_lemma_1 h16 h17 x2 xx;
+  Hacl.Spec.EC.AddAndDouble.lemma_fdifference_unrolled''' (as_seq h17 zz) (as_seq h17 xx);
+  fdifference zz xx; // red red
+  let h18 = ST.get() in
+  let scalar = (uint64_to_limb Hacl.Bignum.Constants.a24) in
+  Hacl.Spec.EC.AddAndDouble.fscalar_is_fine (as_seq h18 zz) scalar;
+  fscalar zzz zz scalar;
+  let h19 = ST.get() in
+  lemma_513_is_52 (as_seq h19 xx);
+  no_upd_lemma_1 h17 h18 zz xx;
+  no_upd_lemma_1 h18 h19 zzz xx;
+  Hacl.Spec.EC.AddAndDouble.fsum_52_is_53 (as_seq h19 zzz) (as_seq h19 xx);
+  fsum zzz xx; // red red
+  let h20 = ST.get() in
+  no_upd_lemma_1 h18 h19 zzz zz;
+  no_upd_lemma_1 h19 h20 zzz zz;
+  lemma_5413_is_55 (as_seq h20 zz);
+  Hacl.Spec.EC.AddAndDouble.fmul_53_55_is_fine (as_seq h20 zzz) (as_seq h20 zz);
+  fmul z2 zzz zz
+
+
+
+val fmonty__:
+  tmp:buffer limb{length tmp = 40} ->
+  ppx:felem -> ppz:felem -> ppqx:felem -> ppqz:felem ->
+  px:felem -> pz:felem -> pqx:felem -> pqz:felem ->
+  qx:felem -> Stack unit
+    (requires (fun h ->
+      live h ppx /\ live h ppz /\ live h ppqx /\ live h ppqz
+      /\ live h px /\ live h pz /\ live h pqx /\ live h pqz
+      /\ live h qx /\ live h tmp
+      /\ red_513 (as_seq h px) /\ red_513 (as_seq h pz) /\ red_513 (as_seq h pqx) /\ red_513 (as_seq h pqz)
+      /\ red_513 (as_seq h qx)
+      /\ all_disjoint ppx ppz ppqx ppqz px pz pqx pqz qx
+      /\ same_frame ppx ppz ppqx ppqz px pz pqx pqz
+      /\ frameOf ppx <> frameOf tmp /\ frameOf ppx <> frameOf qx /\ frameOf qx <> frameOf tmp))
+    (ensures (fun h0 _ h1 ->
+      live h0 ppx /\ live h0 ppz /\ live h0 ppqx /\ live h0 ppqz
+      /\ live h0 px /\ live h0 pz /\ live h0 pqx /\ live h0 pqz
+      /\ live h0 qx /\ live h0 tmp
+      /\ live h1 ppx /\ live h1 ppz /\ live h1 ppqx /\ live h1 ppqz
+      /\ red_513 (as_seq h0 px) /\ red_513 (as_seq h0 pz) /\ red_513 (as_seq h0 pqx) /\ red_513 (as_seq h0 pqz)
+      /\ red_513 (as_seq h0 qx)
+      /\ all_disjoint ppx ppz ppqx ppqz px pz pqx pqz qx
+      /\ red_513 (as_seq h1 ppx) /\ red_513 (as_seq h1 ppz)
+      /\ red_513 (as_seq h1 ppqx) /\ red_513 (as_seq h1 ppqz)
+      /\ (as_seq h1 ppx, as_seq h1 ppz, as_seq h1 ppqx, as_seq h1 ppqz) ==
+          fmonty_tot (as_seq h0 px) (as_seq h0 pz) (as_seq h0 pqx) (as_seq h0 pqz) (as_seq h0 qx)
+    ))
+#set-options "--initial_fuel 0 --max_fuel 0 --z3rlimit 10"
+let fmonty__ buf x2 z2 x3 z3 x z xprime zprime qx =
+  let origx      = Buffer.sub buf 0ul  5ul in
+  let origxprime = Buffer.sub buf 5ul  5ul in
+  let zzz        = Buffer.sub buf 10ul 5ul in
+  let xx         = Buffer.sub buf 15ul 5ul in
+  let zz         = Buffer.sub buf 20ul 5ul in
+  let xxprime    = Buffer.sub buf 25ul 5ul in
+  let zzprime    = Buffer.sub buf 30ul 5ul in
+  let zzzprime   = Buffer.sub buf 35ul 5ul in
+  let h0 = ST.get() in
+  fmonty__1 buf x2 z2 x3 z3 x z xprime zprime qx;
+  let h1 = ST.get() in
+  fmonty__2 buf x2 z2 x3 z3 x z xprime zprime qx;
+  let h2 = ST.get() in
+  fmonty__3 buf x2 z2 x3 z3 x z xprime zprime qx;
+  let h3 = ST.get() in
+  lemma_fmonty_split (as_seq h0 x) (as_seq h0 z) (as_seq h0 xprime) (as_seq h0 zprime) (as_seq h0 qx);
+  ()
+  (* let h0 = ST.get() in *)
+  (* blit x 0ul origx 0ul 5ul; *)
+  (* let h1 = ST.get() in *)
+  (* Hacl.Spec.Bignum.Fmul.lemma_whole_slice (as_seq h0 x); *)
+  (* Hacl.Spec.Bignum.Fmul.lemma_whole_slice (as_seq h1 origx); *)
+  (* Hacl.Spec.EC.AddAndDouble.fsum_513_is_53 (as_seq h1 x) (as_seq h1 z); *)
+  (* fsum x z; // x < x + z *)
+  (* let h2 = ST.get() in *)
+  (* Hacl.Spec.EC.AddAndDouble.lemma_fdifference_unrolled'' (as_seq h2 z) (as_seq h2 origx); *)
+  (* Hacl.Spec.EC.AddAndDouble.lemma_fdifference_unrolled''' (as_seq h2 z) (as_seq h2 origx); *)
+  (* fdifference z origx; // z <- 8p + x - z *)
+  (* let h3 = ST.get() in *)
+  (* blit xprime 0ul origxprime 0ul 5ul; *)
+  (* let h4 = ST.get() in *)
+  (* Hacl.Spec.Bignum.Fmul.lemma_whole_slice (as_seq h3 xprime); *)
+  (* Hacl.Spec.Bignum.Fmul.lemma_whole_slice (as_seq h4 origxprime); *)
+  (* Hacl.Spec.EC.AddAndDouble.fsum_513_is_53 (as_seq h4 xprime) (as_seq h4 zprime); *)
+  (* fsum xprime zprime; // xprime <- xprime + zprime *)
+  (* let h5 = ST.get() in *)
+  (* Hacl.Spec.EC.AddAndDouble.lemma_fdifference_unrolled'' (as_seq h5 zprime) (as_seq h5 origxprime); *)
+  (* fdifference zprime origxprime; // zprime <- 8p + xprime - zprime *)
+  (* let h6 = ST.get() in *)
+  (* Hacl.Spec.EC.AddAndDouble.fmul_53_55_is_fine (as_seq h6 xprime) (as_seq h6 z); *)
+  (* fmul xxprime xprime z; // xxprime <- sum * sub *)
+  (* let h7 = ST.get() in *)
+  (* Hacl.Spec.EC.AddAndDouble.fmul_53_55_is_fine (as_seq h7 x) (as_seq h7 zprime); *)
+  (* fmul zzprime x zprime; // zzprime <- sum * sub *)
+  (* let h8 = ST.get() in *)
+  (* blit xxprime 0ul origxprime 0ul 5ul; *)
+  (* let h9 = ST.get() in *)
+  (* Hacl.Spec.Bignum.Fmul.lemma_whole_slice (as_seq h8 xxprime); *)
+  (* Hacl.Spec.Bignum.Fmul.lemma_whole_slice (as_seq h9 origxprime); *)
+  (* Hacl.Spec.EC.AddAndDouble.fsum_513_is_53 (as_seq h9 xxprime) (as_seq h9 zzprime); *)
+  (* fsum xxprime zzprime; // xxprime <- sum *)
+  (* let h10 = ST.get() in *)
+  (* Hacl.Spec.EC.AddAndDouble.lemma_fdifference_unrolled''' (as_seq h10 zzprime) (as_seq h10 origxprime); *)
+  (* fdifference zzprime origxprime; // zzprime <- sub *)
+  (* let h11 = ST.get() in *)
+  (* lemma_53_is_5413 (as_seq h11 xxprime); *)
+  (* Hacl.Spec.Bignum.Fsquare.fsquare_5413_is_fine (as_seq h11 xxprime); *)
+  (* fsquare_times x3 xxprime 1ul; // sum sum *)
+  (* let h12 = ST.get() in *)
+  (* lemma_53_is_5413 (as_seq h12 zzprime); *)
+  (* Hacl.Spec.Bignum.Fsquare.fsquare_5413_is_fine (as_seq h12 zzprime); *)
+  (* fsquare_times zzzprime zzprime 1ul; // sub sub *)
+  (* let h13 = ST.get() in *)
+  (* lemma_513_is_53 (as_seq h13 zzzprime); lemma_513_is_55 (as_seq h13 qx); *)
+  (* fmul z3 zzzprime qx; *)
+  (* let h14 = ST.get() in *)
+  (* lemma_53_is_5413 (as_seq h14 x); *)
+  (* Hacl.Spec.Bignum.Fsquare.fsquare_5413_is_fine (as_seq h14 x); *)
+  (* fsquare_times xx x 1ul; // sum red *)
+  (* let h15 = ST.get() in *)
+  (* Hacl.Spec.Bignum.Fsquare.fsquare_5413_is_fine (as_seq h15 z); *)
+  (* fsquare_times zz z 1ul; // red sub *)
+  (* let h16 = ST.get() in *)
+  (* lemma_513_is_53 (as_seq h16 xx); *)
+  (* lemma_513_is_55 (as_seq h16 zz); *)
+  (* Hacl.Spec.EC.AddAndDouble.fmul_53_55_is_fine (as_seq h16 xx)  (as_seq h16 zz); *)
+  (* fmul x2 xx zz; // red red *)
+  (* let h17 = ST.get() in *)
+  (* Hacl.Spec.EC.AddAndDouble.lemma_fdifference_unrolled'' (as_seq h17 zz) (as_seq h17 xx); *)
+  (* fdifference zz xx; // red red *)
+  (* let h18 = ST.get() in *)
+  (* let scalar = (uint64_to_limb Hacl.Bignum.Constants.a24) in *)
+  (* Hacl.Spec.EC.AddAndDouble.fscalar_is_fine (as_seq h18 zz) scalar; *)
+  (* fscalar zzz zz scalar; *)
+  (* let h19 = ST.get() in *)
+  (* lemma_513_is_52 (as_seq h19 xx); *)
+  (* Hacl.Spec.EC.AddAndDouble.fsum_52_is_53 (as_seq h19 zzz) (as_seq h19 xx); *)
+  (* fsum zzz xx; // red red *)
+  (* let h20 = ST.get() in *)
+  (* Hacl.Spec.EC.AddAndDouble.fmul_53_55_is_fine (as_seq h20 zzz) (as_seq h20 zz); *)
+  (* fmul z2 zzz zz; *)
+  (* pop_frame(); *)
+  (* admit() *)
+
+
+#set-options "--initial_fuel 0 --max_fuel 0 --z3rlimit 10"
 
 val fmonty_:
   ppx:felem -> ppz:felem -> ppqx:felem -> ppqz:felem ->
@@ -180,7 +573,7 @@ val fmonty_:
       /\ (as_seq h1 ppx, as_seq h1 ppz, as_seq h1 ppqx, as_seq h1 ppqz) ==
           fmonty_tot (as_seq h0 px) (as_seq h0 pz) (as_seq h0 pqx) (as_seq h0 pqz) (as_seq h0 qx)
     ))
-#set-options "--initial_fuel 0 --max_fuel 0 --z3rlimit 1000"
+#set-options "--initial_fuel 0 --max_fuel 0 --z3rlimit 10"
 let fmonty_ x2 z2 x3 z3 x z xprime zprime qx =
   push_frame();
   let buf = create limb_zero 40ul in
@@ -253,14 +646,15 @@ let fmonty_ x2 z2 x3 z3 x z xprime zprime qx =
   Hacl.Spec.EC.AddAndDouble.fmul_53_55_is_fine (as_seq h16 xx)  (as_seq h16 zz);
   fmul x2 xx zz; // red red
   let h17 = ST.get() in
-  Hacl.Spec.EC.AddAndDouble.lemma_fdifference_unrolled'' (as_seq h17 zz) (as_seq h17 xx);  
+  Hacl.Spec.EC.AddAndDouble.lemma_fdifference_unrolled'' (as_seq h17 zz) (as_seq h17 xx);
   fdifference zz xx; // red red
   let h18 = ST.get() in
   let scalar = (uint64_to_limb Hacl.Bignum.Constants.a24) in
   Hacl.Spec.EC.AddAndDouble.fscalar_is_fine (as_seq h18 zz) scalar;
   fscalar zzz zz scalar;
   let h19 = ST.get() in
-  Hacl.Spec.EC.AddAndDouble.fsum_513_is_53 (as_seq h19 zzz) (as_seq h19 xx);
+  lemma_513_is_52 (as_seq h19 xx);
+  Hacl.Spec.EC.AddAndDouble.fsum_52_is_53 (as_seq h19 zzz) (as_seq h19 xx);
   fsum zzz xx; // red red
   let h20 = ST.get() in
   Hacl.Spec.EC.AddAndDouble.fmul_53_55_is_fine (as_seq h20 zzz) (as_seq h20 zz);
