crypto/bignum/x25519/Hacl.Spec.EC.AddAndDouble2.fst
@@ -11,12 +11,19 @@ open Hacl.Spec.EC.AddAndDouble
 #set-options "--initial_fuel 0 --max_fuel 0 --z3rlimit 10"
 
 let s_513 = s:seqelem{red_513 s}
+let s_52 = s:seqelem{red_52 s}
+let s_53 = s:seqelem{red_53 s}
+let s_5413 = s:seqelem{red_5413 s}
 
 let lemma_53_is_5413 (s:seqelem{red_53 s}) : Lemma (red_5413 s) = ()
 let lemma_513_is_53 (s:seqelem{red_513 s}) : Lemma (red_53 s) = ()
 let lemma_513_is_55 (s:seqelem{red_513 s}) : Lemma (red_55 s) = ()
 let lemma_513_is_5413 (s:seqelem{red_513 s}) : Lemma (red_5413 s) = ()
 let lemma_513_is_52 (s:seqelem{red_513 s}) : Lemma (red_52 s) = ()
+let lemma_5413_is_55 (s:seqelem{red_5413 s}) : Lemma (Hacl.Spec.EC.AddAndDouble.red_55 s) = ()
+
+
+#reset-options "--initial_fuel 0 --max_fuel 0 --z3rlimit 10"
 
 val fmonty_tot:
   px:s_513 -> pz:s_513 ->
@@ -39,8 +46,8 @@ let fmonty_tot px pz pqx pqz qx =
   let zzprime = fmul_tot px' pqz' in
   fsum_513_is_53 xxprime zzprime;
   let xxprime' = fsum_tot xxprime zzprime in
-  lemma_fdifference_unrolled''' zzprime pqx;
-  let zzprime' = fdifference_tot zzprime pqx in
+  lemma_fdifference_unrolled''' zzprime xxprime;
+  let zzprime' = fdifference_tot zzprime xxprime in
   lemma_53_is_5413 xxprime';
   fsquare_5413_is_fine xxprime';
   let x3 = fsquare_times_tot xxprime' 1 in
@@ -58,13 +65,89 @@ let fmonty_tot px pz pqx pqz qx =
   lemma_513_is_55 zz;
   fmul_53_55_is_fine xx zz;
   let x2 = fmul_tot xx zz in
-  lemma_fdifference_unrolled'' zz xx;  
+  lemma_fdifference_unrolled''' zz xx;
   let zz' = fdifference_tot zz xx in
   let scalar = (uint64_to_limb Hacl.Bignum.Constants.a24) in
-  fscalar_is_fine zz scalar;
-  let zzz = fscalar_tot zz (uint64_to_limb Hacl.Bignum.Constants.a24) in
-  fsum_513_is_53 zzz xx;
+  fscalar_is_fine zz' scalar;
+  let zzz = fscalar_tot zz' scalar in
+  lemma_513_is_52 xx;
+  fsum_52_is_53 zzz xx;
   let zzz' = fsum_tot zzz xx in
+  lemma_5413_is_55 zz';
   fmul_53_55_is_fine zzz' zz';
   let z2 = fmul_tot zzz' zz' in
   (x2, z2, x3, z3)
+
+
+val fmonty_tot_1:
+  px:s_513 -> pz:s_513 ->
+  pqx:s_513 -> pqz:s_513 ->
+  qx:s_513 ->
+  Tot (s_53 * s_5413 * s_513 * s_513)
+let fmonty_tot_1 px pz pqx pqz qx =
+  fsum_513_is_53 px pz;
+  let px' = fsum_tot px pz in
+  lemma_fdifference_unrolled'' pz px;
+  lemma_fdifference_unrolled''' pz px;
+  let pz' = fdifference_tot pz px in
+  fsum_513_is_53 pqx pqz;
+  let pqx' = fsum_tot pqx pqz in
+  lemma_fdifference_unrolled'' pqz pqx;
+  let pqz' = fdifference_tot pqz pqx in
+  fmul_53_55_is_fine pqx' pz';
+  let xxprime = fmul_tot pqx' pz' in
+  fmul_53_55_is_fine px' pqz';
+  let zzprime = fmul_tot px' pqz' in
+  px', pz', xxprime, zzprime
+
+
+val fmonty_tot_2:
+  px':s_53 -> pz':s_5413 -> qx:s_513 -> xxprime:s_513 -> zzprime:s_513 ->
+  Tot (s_513 * s_513 * s_513 * s_513)
+let fmonty_tot_2 px' pz' qx xxprime zzprime =
+  fsum_513_is_53 xxprime zzprime;
+  let xxprime' = fsum_tot xxprime zzprime in
+  lemma_fdifference_unrolled''' zzprime xxprime;
+  let zzprime' = fdifference_tot zzprime xxprime in
+  lemma_53_is_5413 xxprime';
+  fsquare_5413_is_fine xxprime';
+  let x3 = fsquare_times_tot xxprime' 1 in
+  fsquare_5413_is_fine zzprime';
+  let zzzprime = fsquare_times_tot zzprime' 1 in
+  lemma_513_is_53 zzzprime; lemma_513_is_55 qx;
+  fmul_53_55_is_fine zzzprime qx;
+  let z3 = fmul_tot zzzprime qx in
+  lemma_53_is_5413 px';
+  fsquare_5413_is_fine px';
+  let xx = fsquare_times_tot px' 1 in
+  fsquare_5413_is_fine pz';
+  let zz = fsquare_times_tot pz' 1 in
+  x3, z3, xx, zz
+
+
+val fmonty_tot_3: s_513 -> s_513 -> s_513 -> s_513 -> Tot (s_513 * s_513 * s_513 * s_513)
+let fmonty_tot_3 x3 z3 xx zz =
+  lemma_513_is_53 xx;
+  lemma_513_is_55 zz;
+  fmul_53_55_is_fine xx zz;
+  let x2 = fmul_tot xx zz in
+  lemma_fdifference_unrolled''' zz xx;
+  let zz' = fdifference_tot zz xx in
+  let scalar = (uint64_to_limb Hacl.Bignum.Constants.a24) in
+  fscalar_is_fine zz' scalar;
+  let zzz = fscalar_tot zz' scalar in
+  lemma_513_is_52 xx;
+  fsum_52_is_53 zzz xx;
+  let zzz' = fsum_tot zzz xx in
+  lemma_5413_is_55 zz';
+  fmul_53_55_is_fine zzz' zz';
+  let z2 = fmul_tot zzz' zz' in
+  (x2, z2, x3, z3)
+
+
+val lemma_fmonty_split:   px:s_513 -> pz:s_513 -> pqx:s_513 -> pqz:s_513 -> qx:s_513 ->
+  Lemma (let px', pz', xxprime, zzprime = fmonty_tot_1 px pz pqx pqz qx in
+    let x3, z3, xx, zz = fmonty_tot_2 px' pz' qx xxprime zzprime in
+    let x2, z2, x3, z3 = fmonty_tot_3 x3 z3 xx zz in
+    (x2, z2, x3, z3) == fmonty_tot px pz pqx pqz qx)
+let lemma_fmonty_split px pz pqx pqz qx = ()
